\documentclass[../skript.tex]{subfiles}

\begin{document}
Consider the following special case:
\begin{problem}
\begin{equation}
\tag{$P$}
\begin{IEEEeqnarraybox}[][c]{c}
\min \frac{1}{2} \| y - y_d \|^2 + \frac{\lambda}{2} \| u \|^2 \\
\begin{IEEEeqnarraybox}[][c]{rCl}
\lapl y &=& u \\
y &=& 0
\end{IEEEeqnarraybox} \\
y_a \leq y(x) \leq y_b \quad \forall x \in \bar{\Omega}
\end{IEEEeqnarraybox}
\end{equation}
Here, let $\Omega \subseteq \R^2$ be polygonal and convex.
For simplicity let $y_a, y_b \in \R$ and
\[
	y_a < 0 < y_b.
\]
\end{problem}
In this setting one has $\bar{y} \in H_0^1$ and
\[
	(\nabla \bar{y}, \nabla \varphi) = (\bar{u}, \varphi) \quad \forall \varphi \in H_0^1.
\]
Furthermore, one seeks $\bar{p} \in C^2$ with
\[
	- (\bar{p}, \lapl \varphi) = (\bar{y} - y_d, \varphi) + \langle \bar{\mu}_b - \bar{\mu}_a, \varphi \rangle \quad \forall \varphi \in H_0^1 \cap H^2 \hookrightarrow C(\Omega)
\]
and
\[
	\lambda \bar{u} + \bar{p} = 0.
\]
For the Lagrange multipliers, we have $\bar{\mu}_a, \bar{\mu}_b \geq 0$
\[
\langle \bar{\mu}_a, y_a - \bar{y} \rangle = 0 = \langle \bar{\mu}_b, y_b - \bar{y} \rangle.
\]

In the setting $\bar{u} \in L^2$ and one has $\bar{y} \in H_0^1 \cap H^2 \hookrightarrow C(\bar{\Omega})$.
Furthermore $\bar{\mu}_a, \bar{\mu}_b \in M(\Omega)$ imply $\bar{p} \in W^{1, s}$ and $\bar{u} \in W^{1, s}$ for $s < 2$ in 2D.
As of such, one can seek $\bar{p} \in W^{1, s}_0(\Omega)$ with
\[
	(\nabla \bar{p}, \nabla \varphi) = (\bar{y} - y_d, \varphi) + \langle \bar{\mu}_b - \bar{\mu}_a, \varphi \rangle \quad \forall \varphi \in \left(W_0^{1, s} \right)^* \hookrightarrow C(\Omega), s < 2.
\]
This in turn implies
\[
	\bar{u} \in L^p \quad \forall p < \infty.
\]

Consequently, $\bar{y} \in W^{2, p}(\Omega_1)$, for $\Omega_1 \subset\subset \Omega$, a strictly interior subset. 
\begin{theorem}
Under these assumptions (variational discretization, $y_a, y_b \in \R$) we find
\[
	\| \bar{u} - \bar{u}_h \|^2_{L^2} \leq c \left( \| p_1(\bar{u}) - p_{1, h}(\bar{u}) \|_{L^2}^2 + \| p_2(\bar{\mu}) - p_{2, h}(\bar{\mu}) \|^2_{L^2} + \| y(\bar{u}) - y_h(\bar{u}) \|_{L^{\infty}} \right)
\]
where $p_1(\bar{u}) \in H^2 \cap H_0^1$ with
\begin{IEEEeqnarray*}{rCl"l}
(\nabla p_1, \nabla \varphi) &=& (y(u) - y_d, \varphi) & \forall \varphi \in H_0^1 \\
(p_2, \lapl \varphi) &=& \langle \bar{\mu}_b - \bar{\mu}_a, \varphi \rangle & \forall \varphi \in H_0^1 \cap H^2
\end{IEEEeqnarray*}
and $p_{1, h}, p_{2, h}$, respectively, are the finite element approximations of $p_1$ and $p_2$.
\end{theorem}
\begin{proof}
\begin{IEEEeqnarray*}{rCl}
\lambda \| \bar{u} - \bar{u}_h \|_{L^2}^2 &\leq& f_h''(\xi) (\bar{u} - \bar{u}_h, \bar{u} - \bar{u}_h) \\
&=& f_h'(\bar{u})(\bar{u} - \bar{u}_h) - f_h'(\bar{u}_h)(\bar{u}-\bar{u}_h) \\
&=& (\lambda \bar{u} + p_{1, h}(\bar{u}), \bar{u} - \bar{u}_h) - (\lambda \bar{u}_h + p_{1, h}(\bar{u}_h), \bar{u} - \bar{u}_h) \\
&=& (\lambda \bar{u} + p_1(\bar{u}), \bar{u} - \bar{u}_h) - (p_1(\bar{u}) - p_{1, h}(\bar{u}), \bar{u}-\bar{u}_h) \\
&& \quad {} - (\lambda \bar{u}_h + p_{1, h}(\bar{u}_h), \bar{u} - \bar{u}_h))
\end{IEEEeqnarray*}
and because $0 = \lambda \bar{u} + \bar{p} = \lambda \bar{u} + p_1(\bar{u}) + p_2(\bar{\mu})$ one has $\lambda \bar{u} + p_1(\bar{u}) = p_2(\bar{u}) \neq 0$, and this can be transformed into
\begin{IEEEeqnarray*}{rCl}
&=& (- p_2(\bar{\mu}), \bar{u} - \bar{u}_h) - (p_{2, h}(\bar{\mu}_h), \bar{u}-\bar{u}_h) - (p_1(\bar{u}) - p_{1, h}(\bar{u}), \bar{u} - \bar{u}_h) \\
&=& -( p_2(\bar{\mu}) - p_{2, h}(\bar{\mu}), \bar{u} - \bar{u}_h) - (p_{2, h}(\bar{\mu}) - p_{2, h}(\bar{\mu}_h), \bar{u}-\bar{u}_h) \\
&& \quad {} - (p_1(\bar{u}) - p_{1, h}(\bar{u}), \bar{u} - \bar{u}_h)
\end{IEEEeqnarray*}
By Young's inequality, this becomes:
\begin{IEEEeqnarray*}{rCl}
\| \bar{u} - \bar{u}_h \|_{L^2}^2 &\leq& c \Big( \| p_1(\bar{u}) - p_{1, h}(\bar{u}) \|_{L^2}^2 + \| p_2(\bar{\mu}) - p_{2, h}(\bar{\mu}) \|_{L^2}^2 \\
&& \quad {} - (p_{2, h} (\bar{\mu}) - p_{2, h}(\bar{\mu}_h), \bar{u} - \bar{u}_h) \Big)
\end{IEEEeqnarray*}
Consider that by the discrete state equation with the right hand side $\bar{u} - \bar{u}_h$ and tested by $\varphi_h = p_{2, h}(\bar{\mu}) - p_{2, h}(\bar{\mu}_h)$ we have
\begin{IEEEeqnarray*}{rCl}
- (p_{2, h} (\bar{\mu}) - p_{2, h}(\bar{\mu}_h), \bar{u} - \bar{u}_h) &=& - (\nabla (y_h(\bar{u}) - y_h(\bar{u}_h)), \nabla (p_{2, h}(\bar{\mu}) - p_{2, h}(\bar{\mu}_h))) \\
&=& \underbrace{ \langle y_h(\bar{u}_h) - y_h(\bar{u}), \bar{\mu}_b - \bar{\mu}_a \rangle }_{\text{(I)}} + \underbrace{ \langle y_h(\bar{u}) - y_h(\bar{u}_h), \bar{\mu}_{b, h} - \bar{\mu}_{a, h} \rangle }_{\text{(II)}}
\end{IEEEeqnarray*}
We first consider (I):
\begin{IEEEeqnarray*}{rCl}
\langle y_h(\bar{u}_h) - y_h(\bar{u}), \bar{\mu}_b - \bar{\mu}_a \rangle &=& \langle \underbrace{ y_h(\bar{u}_h) }_{= \bar{y}_h \leq y_b} - y_h(\bar{u}), \bar{\mu}_b \rangle - \langle y_h(\bar{u}_h) - y_h(\bar{u}), \bar{\mu}_a \rangle
\end{IEEEeqnarray*}
Let's discuss the first term on the right hand side:
\begin{IEEEeqnarray*}{rCl}
\langle y_h(\bar{u}_h) - y_h(\bar{u}), \bar{\mu}_b \rangle &=& \langle \underbrace{ y_h(\bar{u}_h) - y_b }_{\leq 0} + y_b - y_h(\bar{u}), \underbrace{ \bar{\mu}_b }_{\geq 0} \rangle \\
&\leq& \langle y_b - y_h(\bar{u}), \bar{\mu}_b \rangle \\
&=& \langle y_b - \underbrace{y(\bar{u})}_{= \bar{y}} + y(\bar{u}) - y_h(\bar{u}), \bar{\mu}_b \rangle \\
&=& \underbrace{ \langle y_b - \bar{y}, \bar{\mu}_b \rangle }_{=0} + \langle y(\bar{u}) - y_h(\bar{u}), \bar{\mu}_b \rangle \\
&=& \langle y(\bar{u}) - y_h(\bar{u}), \bar{\mu}_b \rangle_{C, C^*} \\
&\leq& \| y(\bar{u}) - y_h(\bar{u}) \|_{L^\infty} \| \bar{\mu}_b \|_{M}
\end{IEEEeqnarray*}
The second term can be estimated in the same manner:
\[
	- \langle y_h(\bar{u}_h) - y_h(\bar{u}), \bar{\mu}_a \rangle \leq \| y(\bar{u}) - y_h(\bar{u}) \|_{L^\infty} \| \bar{\mu}_a \|_{M}.
\]
On the other hand, one obtains for (II):
\[
\langle y_h(\bar{u}) - y_h(\bar{u}_h), \bar{\mu}_{b, h} - \bar{\mu}_{a, h} \rangle \leq \| y(\bar{u}) - y_h(\bar{u}) \|_{L^\infty} \underbrace{ \left( \| \bar{\mu}_{b, h} \|_M + \| \bar{\mu}_{a, h} \|_{M} \right) }_{\leq C},
\]
with $C$ independent of $h$ (this was the previously proven auxiliary result).

Plugging this into our earlier estimate, we have proven so far, that
\begin{IEEEeqnarray*}{rCl}
\| \bar{u} - \bar{u}_h \|_{L^2}^2 &\leq& c \left( \| p_1(\bar{u}) - p_{1, h}(\bar{u}) \|_{L^2}^2 + \| p_2(\bar{\mu}) - p_{2, h}(\bar{\mu}) \|_{L^2}^2 \right) \\
&& \quad {} + c \| y(\bar{u}) - y_h(\bar{u}) \|_{L^\infty}
\end{IEEEeqnarray*}
\begin{itemize}
\item Now, by our previous finite element error results we have
\begin{IEEEeqnarray*}{rCl}
\| p_1(\bar{u}) - p_{1, h}(\bar{u}) \|_{L^2}^2 &\leq& ch^2 \| \nabla^2 p_1(\bar{u}) \| \\
&\leq& ch^2 \| y(\bar{u}) - y_a \|_{L^2} \\
&\leq& ch^2 \left( \| \bar{u} \|_{L^2} + \| y_a \|_{L^2} \right)
\end{IEEEeqnarray*}
\item Furthermore, Casas has proven (see \cite{HinzePinnauUlbrich}) that
\[
	\| p_2(\bar{\mu}) - p_{2, h}(\bar{\mu}) \|_{L^2} \leq ch^{2 - \frac{d}{2} - \delta} \| \bar{\mu} \|_{M(\Omega)},
\]
with $\delta > 0$.
For the case $d = 2$ this gives:
\[
	\| p_2(\bar{\mu}) - p_{2, h}(\bar{\mu}) \|_{L^2} \leq ch^{1 - \delta} \| \bar{\mu} \|_{M(\Omega)}.
\]
\item Lastly, it holds (again, see \cite{HinzePinnauUlbrich}) that $\bar{u} \in W^{1, s}$, where $s < \infty$ for $d = 2$ and $s < 3$ for $d = 3$ as well as
\[
	\| y(\bar{u}) - y_h(\bar{u}) \|_{L^\infty} \leq c h^{4 - d - \delta} \| \bar{u} \|_{W^{1, s}},
\]
again with $\delta > 0$.
In our case $d = 2$, this gives
\[
	\| y(\bar{u}) - y_h(\bar{u}) \|_{L^\infty} \leq c h^{2 - \delta} \| \bar{u} \|_{W^{1, s}},
\]
\end{itemize}
With these results, we obtain
\[
	\| \bar{u} - \bar{u}_h \|_{L^2}^2 \leq c \left( h^4 + h^{2 - \varepsilon} + h^{2 - \delta} \right)
\]
and this in 2D:
\[
	\| \bar{u} - \bar{u}_h \|_{L^2}^2 \leq c h^{1 - \varepsilon}.
\]
\end{proof}
\end{document}