\documentclass[../skript.tex]{subfiles}

\begin{document}
Firstly, the existence of a globally optimal control $\bar{u}_h^r$ of \cref{eq:Phr} is immediately clear.
\begin{proof}[convergence]
Recall the proof for convex problems:
\begin{itemize}
\item $f'(\bar{u})(u - \bar{u}) \geq 0 \quad \forall u \in U_{ad}$
\item $f'_h(\bar{u}_h)(u_h - \bar{u}_h) \geq 0 \quad \forall u_h \in U_{ad,h}$
\end{itemize}
Because $\bar{u}_h$ was admissible for the first equation and $\bar{u}$ was admissible for the second (variational discretization):
\begin{itemize}
\item $f'(\bar{u})(\bar{u}_h - \bar{u}) \geq 0$
\item $f'_h(\bar{u}_h)(\bar{u} - \bar{u}_h) \geq 0$
\end{itemize}
Furthermore, we needed
\[
\lambda \| \bar{u} - \bar{u}_h \|^2 \leq f_h''(u_\xi)(\bar{u}_h - \bar{u})^2. 
\]
This condition we do not have, but we have second order sufficient conditions. We used that equality to estimate via an intermediate value theorem:
\begin{IEEEeqnarray*}{rCl}
\lambda \| \bar{u}_h  - \bar{u} \|^2 &\leq& f_h''(u_\xi)(\bar{u} - \bar{u}_h)^2 \\
&=& \underbrace{ - f_h'(\bar{u}_h)(\bar{u} - \bar{u}_h) }_{\leq 0} + f_h'(\bar{u})(\bar{u} - \bar{u}_h) \\
&\leq& - f'(\bar{u})(\bar{u} - \bar{u}_h) + f_h'(\bar{u})(\bar{u} - \bar{u}_h) \\
&\vdots& \\
&\leq& ch^2(\ldots) \| \bar{u} - \bar{u}_h \|
\end{IEEEeqnarray*}

In the non-convex case, the equations
\begin{itemize}
\item $f'(\bar{u})(\bar{u}_h - \bar{u}) \geq 0$
\item $f'_h(\bar{u}_h)(\bar{u} - \bar{u}_h) \geq 0$
\end{itemize}
still hold.
By second order sufficient conditions we have
\[
\delta \| \bar{u} - \bar{u}_h^r \|^2 \leq f''(\bar{u})(\bar{u} - \bar{u}_h^r)^2.
\]
Unlike in the convex case, this holds for $f$ and not for $f_h$.

Comparing to the convex proof, we would like to estimate
\begin{IEEEeqnarray*}{rCl}
f_h''(u_\xi)(\bar{u} - \bar{u}_h)^2 &=& f_h'(\bar{u}) (\bar{u} - \bar{u}_h^r) - f_h'(\bar{u}_h^r)(\bar{u} - \bar{u}_h^r) \\
&\leq& f'(\bar{u})(\bar{u} - \bar{u}_h^r) - f_h'(\bar{u})(\bar{u} - \bar{u}_h^r) \\
&\leq& ?
\end{IEEEeqnarray*}
We still have to show that we can estimate $\delta \| \bar{u} - \bar{u}_h^r \|^2$ by $f_h''(u_\xi)(\bar{u} - \bar{u}_h)^2$ and then have to finish up the estimate.

By the second order sufficient conditions, we know
\[
	f''(\bar{u}) (\underbrace{\bar{u}_h^r - \bar{u}}_{v})^2 \geq \delta \| \underbrace{\bar{u}_h^r - \bar{u}}_{v} \|^2
\]
Since we use the mean value theorem and $\bar{u}_h^r$ and $\bar{u}_h$ have distance at most $r$, we work with ``$u$ close enough to $\bar{u}$'' and ``$h$ small enough''.
\begin{IEEEeqnarray*}{rCl}
f_h''(u)v^2 &=& \underbrace{\left( f''_h(u) v^2 - f''(u) v^2 \right)}_{\text{FE error}} + \underbrace{\left( f''(u) v^2 - f''(\bar{u}) v^2 \right)}_{\text{Lipschitz continuity}} + \underbrace{ f''(\bar{u}) v^2 }_{\geq \delta \| v \|^2_{L^2(\Omega)}}
\end{IEEEeqnarray*}
Of course, we don't have either result yet, but that's how we plan to estimate them. For the first term:
\begin{IEEEeqnarray*}{rCl}
f_h''(u) v^2 - f''(u) v^2 &=& \| G_h'(u) v \|^2 - \| G'(u) v \|^2\\
&& {} + \int_\Omega p(y(u)) d_{yy} (G(u)) (G'(u)v)^2 \\
&& \qquad {} - p_h(y_h(u)) d_{yy}(G_h(u)) (G_h'(u)v)^2 \dx
\end{IEEEeqnarray*}
As of such we need to estimate the terms on the right hand side:
\begin{IEEEeqnarray*}{rCl}
\| G_h'(u) v \|^2 - \| G'(u) v \|^2 &=& \int_\Omega \left( G_h'(u)v + G'(u)v \right) \left( G_h'(u)v - G'(u) v \right) \dx \\
&\leq& \| G_h'(u)v + G'(u) v \| \| G_h'(u) v - G'(u) v \|
\end{IEEEeqnarray*}
The linearized state equation was (omitting boundary conditions here):
\[
	- \lapl \tilde{y} + d_y(y) \tilde{y} = 0
\]
or in the weak form:
\[
	(\nabla \tilde{y}, \nabla v) + (d_y(y)\tilde{y}, v) = (u, v) \quad \forall v \in V,
\]
and analogously for the discrete case:
\[
	(\nabla \tilde{y}_h, \nabla v) + (d_y(y_h)\tilde{y}_h, v) = (u, v) \quad \forall v \in V_h.
\]
Hence, we consider the intermediate equation
\[
	(\nabla  z, \nabla v) + (d_y(y_h) z, v) = (u, v) \quad \forall v \in V
\]
Recall that we want to estimate $\tilde{y}_h - \tilde{y}$:
\begin{IEEEeqnarray*}{rCl}
\| \tilde{y}_h - \tilde{y} \| &\leq& \underbrace{ \| \tilde{y}_h - z \| }_{\leq Ch^2} + \| z - \tilde{y} \|
\end{IEEEeqnarray*}
For the other term:
\[
	- \lapl (z - \tilde{y}) + d_y(y_h) z - d_y(y) \tilde{y} = 0
\]
or by adding another zero:
\[
	- \lapl (z - \tilde{y}) + d_y(y_h) (z - \tilde{y}) = (d_y(y)- d_y(y_h)) \tilde{y}.
\]
This yields:
\[
	\| z - \tilde{y} \| \leq c \| (d_y(y) - d_y(y_h)) \tilde{y} \|
\]
By assumption $d$ was Lipschitz continuous up to order 2 and $\tilde{y}$ is a PDE with $y$ on the right hand side. Thus:
\begin{IEEEeqnarray*}{rCl}
	\| z - \tilde{y} \| \leq c \| (d_y(y) - d_y(y_h)) \tilde{y} \| &\leq& c \| \tilde{y} \|_{L^\infty} \| d_y(y) - d_y(y_h) \| \\
	&\leq& c \| v \| \| y - y_h \|
\end{IEEEeqnarray*}
The term $\| y - y_h \|$ is a formal Finite Element error. One has to estimate it, still - this is doable using similar techniques as in the previous cases. It can be shown however, that it can be estimated against $ch^2 \| v \|$.

% Recall for $\| y - y_h \|$ that we have
% \begin{IEEEeqnarray*}{rCl"l}
% (\nabla y, \nabla v) + (d(y), v) &=& (u, v) & \forall v \in V \\
% (\nabla y_h, \nabla v_h) + (d(y_h), v_h) &=& (u, v_h) & \forall v_h \in V
% \end{IEEEeqnarray*}
% Let us look at the difference:
% \[
% 	(\nabla(y - y_h), \nabla v_h) + (d(y), v_h) - (d(y_h), v_h) = 0 \quad \forall v_h \in V_h
% \]
% Again via a Taylor type argument:
% \[
% 	(\nabla(y - y_h), \nabla v_h) + (d_y(y_\xi)(y - y_h), v_h) = 
% \]

We still need to estimate
\[
	\int_\Omega p d_{yy} (G(u)) (G'(u)v)^2 - p_h d_{yy} (G_h(u)) (G_h'(u) v)^2.
\]
For this one, one has to insert a lot of zeros, for instance
\begin{IEEEeqnarray*}{l}
	\int_\Omega p d_{yy} (G(u)) G'(u)v^2 - p_h d_{yy} (G_h(u)) (G_h'(u) v)^2 \\
	\begin{IEEEeqnarraybox}{Cl}
		=& \int_\Omega (d_{yy}(G(u)) - d_{yy}(G_h(u))) p(G'(u)v)^2 \\
		& {} + \int_\Omega d_{yy} (G_h(u)) (p(G'(u) v)^2 - p_h(G'_h(u) v)^2)
	\end{IEEEeqnarraybox}
\end{IEEEeqnarray*}
Going on:
\begin{IEEEeqnarray*}{rCl}
\int_\Omega p(G'(u) v)^2 - p_h(G'_h(u) v)^2 &=& \int_\Omega (p - p_h) (G'(u)v)^2 + \int_\Omega p_h((G'(u)v)^2 - (G_h'(u) v)^2)
\end{IEEEeqnarray*}
After a couple of further calculations, one arrives at $ch^2 \| v \|^2$.

This estimates the term
\[
f''_h(u) v^2 - f''(u) v^2 \leq ch^2 \| v \|^2.
\]
Repeating the same calculations slightly different for the second term, one obtains
\[
	f''(u) v^2 - f''(\bar{u}) v^2 \leq c \| u - \bar{u} \|  \| v \|^2
\]
We have $c \| u - \bar{u} \| \leq r \leq \delta/4$. By making $h$ small enough, one has $Ch^2 \leq \delta/4$ as well. This gives
\[
	f_h''(u)v^2 \geq \frac{\delta}{2} \| v \|_{L^2(\Omega)}^2.
\]
Going back, we have shown
\[
\frac{\delta}{2} \| \bar{u} - \bar{u}_h^r \|^2 \leq f_h''(u_\xi)(\bar{u} - \bar{u}_h)^2.
\]

One can show furthermore that
\[
f'(\bar{u})(\bar{u} - \bar{u}_h^r) - f_h'(\bar{u})(\bar{u} - \bar{u}_h^r) \leq ch^2 \| \bar{u} - \bar{u}_h^r \|.
\]
\end{proof}
\end{document}